\documentclass[12pt]{article}

\usepackage{amsmath, amssymb}
\usepackage{graphicx}
\usepackage{geometry}
\usepackage{float}

\geometry{margin=1in}

\title{ODE HW 1}
\author{
Greyson Knippel \\[4pt]
MATH 260-1 --- Gonzaga University \\[4pt]
Professor Jensen
}
\date{\today}



\begin{document}

\maketitle


\section*{problem 6}

Show that the function
\[
y(t) = \frac{4}{1 + Ce^{-4t}}, \quad C = 1,2,\dots,5
\]
is a general solution of the differential equation
\[
y' = y(4 - y).
\]


\section*{solution}

rewrite so we dont have to divide.
\[
y = 4(1 + Ce^{-4t})^{-1}.
\]

differentiate using chain rule and power rule.
\[
y' = 4(-1)(1 + Ce^{-4t})^{-2} \cdot \frac{d}{dt}(1 + Ce^{-4t}).
\]

since
\[
\frac{d}{dt}(1 + Ce^{-4t}) = -4Ce^{-4t},
\]
we obtain
\[
y' = \frac{16Ce^{-4t}}{(1 + Ce^{-4t})^2}.
\]

now compute \( y(4 - y) \):
\[
4 - y = 4 - \frac{4}{1 + Ce^{-4t}}
      = \frac{4Ce^{-4t}}{1 + Ce^{-4t}}.
\]

thus,
\[
y(4 - y)
= \frac{4}{1 + Ce^{-4t}} \cdot \frac{4Ce^{-4t}}{1 + Ce^{-4t}}
= \frac{16Ce^{-4t}}{(1 + Ce^{-4t})^2}.
\]

since \( y' = y(4 - y) \), the function satisfies the differential equation.
therefore, \( y(t) = \frac{4}{1 + Ce^{-4t}} \) is a general solution.


\section*{MATLAB plot}

\begin{figure}[H]
\centering
\includegraphics[width=0.8\textwidth]{Figure_1.png}
\caption{Solutions of the differential equation $y' = y(4 - y)$
for $C = 1,2,\dots,5$.}
\end{figure}


\section*{problem 7}
A general solution may fail to produce all solutions of a
differential equation. In Problem 6, show that y = 0 is a
solution of the differential equation, but no value of C in
the given general solution will produce this solution.

\section*{solution}

Take
\[
y(t) = 0.
\]
Then
\[
y'(t) = 0,
\]
and substituting into the differential equation gives
\[
y(4 - y) = 0 \cdot (4 - 0) = 0.
\]
Since \(y' = y(4 - y)\), the constant function \(y = 0\) satisfies the differential equation.


\[
\]
The constant function \(y = 0\) satisfies the differential equation but cannot be 
obtained from the general solution because no value of 
\(C\) makes \(\frac{4}{1 + Ce^{-4t}} = 0\).

\section*{problem 11}
show that 




\end{document}